proof/refine/X64/ArchCSpace1_R.thy
@@ -242,14 +242,14 @@ lemma can_be_is[CSpace1_R_assms]:
   apply (auto simp: Let_def)[1]
   done
 
-lemma maskCap_valid[simp]:
+lemma maskCap_valid[CSpace1_R_assms, simp]:
   "s \<turnstile>' global.maskCapRights R cap = s \<turnstile>' cap"
   by (clarsimp simp: valid_cap'_def global.maskCapRights_def isCap_simps
                      capAligned_def X64_H.maskCapRights_def
               split: capability.split arch_capability.split
                cong: if_cong)
 
-lemma cap_map_update_data:
+lemma cap_map_update_data[CSpace1_R_assms]:
   assumes "cap_relation c c'"
   shows   "cap_relation (update_cap_data p x c) (updateCapData p x c')"
 proof -
@@ -294,53 +294,40 @@ qed
 
 lemmas setCTE_typ_ats[wp] = typ_at_lifts[OF setCTE_typ_at']
 
-lemma capASID_update[simp]:
+lemma arch_updateCapData_Master[CSpace1_R_assms]:
+  "Arch.updateCapData P d acap \<noteq> NullCap \<Longrightarrow>
+   capMasterCap (Arch.updateCapData P d acap) = capMasterCap (ArchObjectCap acap)"
+  by (cases acap; simp add: X64_H.updateCapData_def split: if_split_asm)
+
+context begin (* private method *)
+
+private method updateCapData_cases for c =
+  (cases c; simp add: global.updateCapData_def isCap_simps Let_def),
+  (rename_tac arch_capability),
+  (case_tac arch_capability; simp add: X64_H.updateCapData_def isCap_simps Let_def)
+
+lemma capASID_update[CSpace1_R_assms, simp]:
   "capASID (RetypeDecls_H.updateCapData P x c) = capASID c"
   unfolding capASID_def
-  apply (cases c, simp_all add: updateCapData_def isCap_simps Let_def)
-  apply (rename_tac arch_capability)
-  apply (case_tac arch_capability,
-         simp_all add: global.updateCapData_def X64_H.updateCapData_def isCap_simps Let_def)
-  done
+  by (updateCapData_cases c)
 
-lemma cap_vptr_update'[simp]:
+lemma cap_vptr_update'[CSpace1_R_assms, simp]:
   "cap_vptr' (RetypeDecls_H.updateCapData P x c) = cap_vptr' c"
   unfolding capASID_def
-  apply (cases c, simp_all add: updateCapData_def isCap_simps Let_def)
-  apply (rename_tac arch_capability)
-  apply (case_tac arch_capability,
-         simp_all add: global.updateCapData_def X64_H.updateCapData_def isCap_simps Let_def)
-  done
+  by (updateCapData_cases c)
 
-lemma cap_asid_base_update'[simp]:
+lemma cap_asid_base_update'[CSpace1_R_assms, simp]:
   "cap_asid_base' (RetypeDecls_H.updateCapData P x c) = cap_asid_base' c"
   unfolding cap_asid_base'_def
-  apply (cases c, simp_all add: updateCapData_def isCap_simps Let_def)
-  apply (rename_tac arch_capability)
-  apply (case_tac arch_capability,
-         simp_all add: global.updateCapData_def X64_H.updateCapData_def isCap_simps Let_def)
-  done
+  by (updateCapData_cases c)
 
-lemma updateCapData_Master:
-  "updateCapData P d cap \<noteq> NullCap \<Longrightarrow>
-   capMasterCap (updateCapData P d cap) = capMasterCap cap"
-  apply (cases cap, simp_all add: global.updateCapData_def isCap_simps Let_def
-                           split: if_split_asm)
-  apply (rename_tac arch_capability)
-  apply (case_tac arch_capability, simp_all add: X64_H.updateCapData_def)
-  done
-
-lemma updateCapData_Reply:
+lemma updateCapData_Reply[CSpace1_R_assms, simp]:
   "isReplyCap (updateCapData P x c) = isReplyCap c"
-  apply (cases "updateCapData P x c = NullCap")
-   apply (clarsimp simp: gen_isCap_simps)
-   apply (simp add: global.updateCapData_def gen_isCap_simps Let_def)
-  apply (drule updateCapData_Master)
-  apply (rule master_eqI, rule gen_isCap_Master)
-  apply simp
-  done
+  by (updateCapData_cases c)
 
-lemma capASID_mask[simp]:
+end (* context private method *)
+
+lemma capASID_mask[CSpace1_R_assms, simp]:
   "capASID (maskCapRights x c) = capASID c"
   unfolding capASID_def
   apply (cases c, simp_all add: global.maskCapRights_def isCap_simps Let_def)
@@ -349,7 +336,7 @@ lemma capASID_mask[simp]:
          simp_all add: X64_H.maskCapRights_def isCap_simps Let_def)
   done
 
-lemma cap_vptr_mask'[simp]:
+lemma cap_vptr_mask'[CSpace1_R_assms, simp]:
   "cap_vptr' (maskCapRights x c) = cap_vptr' c"
   unfolding cap_vptr'_def
   apply (cases c, simp_all add: global.maskCapRights_def isCap_simps Let_def)
@@ -358,7 +345,7 @@ lemma cap_vptr_mask'[simp]:
          simp_all add: X64_H.maskCapRights_def isCap_simps Let_def)
   done
 
-lemma cap_asid_base_mask'[simp]:
+lemma cap_asid_base_mask'[CSpace1_R_assms, simp]:
   "cap_asid_base' (maskCapRights x c) = cap_asid_base' c"
   unfolding cap_vptr'_def
   apply (cases c, simp_all add: global.maskCapRights_def isCap_simps Let_def)
@@ -560,7 +547,7 @@ lemma arch_gen_refs_cap_relation_Master_eq[CSpace1_R_assms]:
    \<Longrightarrow> arch_gen_refs c = arch_gen_refs c'"
   by (simp split: cap_relation_split_asm arch_cap.split_asm)
 
-lemma descendants_of_update_ztc:
+lemma descendants_of_update_ztc[CSpace1_R_assms]:
   assumes c: "\<And>x. \<lbrakk> m \<turnstile> x \<rightarrow> slot; \<not> P \<rbrakk> \<Longrightarrow>
                   \<exists>cte'. m x = Some cte'
                     \<and> capMasterCap (cteCap cte') \<noteq> capMasterCap (cteCap cte)
@@ -914,16 +901,6 @@ qed
 context Arch begin arch_global_naming
 
 named_theorems CSpace1_R_2_assms
-
-lemma weak_derived_updateCapData:
-  "\<lbrakk> updateCapData P x c \<noteq> NullCap; weak_derived' c c';
-     capBadge (updateCapData P x c) = capBadge c' \<rbrakk>
-  \<Longrightarrow> weak_derived' (updateCapData P x c) c'"
-  apply (clarsimp simp add: weak_derived'_def updateCapData_Master)
-  apply (clarsimp elim: impE dest!: iffD1[OF updateCapData_Reply])
-  apply (clarsimp simp: gen_isCap_simps)
-  apply (clarsimp simp: Let_def gen_isCap_simps global.updateCapData_def)
-  done
 
 lemma updateMDB_pspace_relation[CSpace1_R_2_assms]:
   assumes "(x, s'') \<in> fst (updateMDB p f s')"
